m

DynamoDbEncryption/runtimes/net/Generated/JsonEncryptor/Action.cs
@@ -1,0 +1,51 @@
+// Copyright Amazon.com Inc. or its affiliates. All Rights Reserved.
+// SPDX-License-Identifier: Apache-2.0
+// Do not modify this file. This file is machine generated, and any changes to it will be overwritten.
+using System;
+using AWS.Cryptography.DbEncryptionSDK.DynamoDb.Json;
+namespace AWS.Cryptography.DbEncryptionSDK.DynamoDb.Json
+{
+  public class Action
+  {
+    private AWS.Cryptography.DbEncryptionSDK.StructuredEncryption.CryptoAction _crypto;
+    private AWS.Cryptography.DbEncryptionSDK.DynamoDb.Json.EsdkEncrypt _esdk;
+    private AWS.Cryptography.DbEncryptionSDK.DynamoDb.Json.DbesdkEncrypt _dbesdk;
+    public AWS.Cryptography.DbEncryptionSDK.StructuredEncryption.CryptoAction Crypto
+    {
+      get { return this._crypto; }
+      set { this._crypto = value; }
+    }
+    public bool IsSetCrypto()
+    {
+      return this._crypto != null;
+    }
+    public AWS.Cryptography.DbEncryptionSDK.DynamoDb.Json.EsdkEncrypt Esdk
+    {
+      get { return this._esdk; }
+      set { this._esdk = value; }
+    }
+    public bool IsSetEsdk()
+    {
+      return this._esdk != null;
+    }
+    public AWS.Cryptography.DbEncryptionSDK.DynamoDb.Json.DbesdkEncrypt Dbesdk
+    {
+      get { return this._dbesdk; }
+      set { this._dbesdk = value; }
+    }
+    public bool IsSetDbesdk()
+    {
+      return this._dbesdk != null;
+    }
+    public void Validate()
+    {
+      var numberOfPropertiesSet = Convert.ToUInt16(IsSetCrypto()) +
+      Convert.ToUInt16(IsSetEsdk()) +
+      Convert.ToUInt16(IsSetDbesdk());
+      if (numberOfPropertiesSet == 0) throw new System.ArgumentException("No union value set");
+
+      if (numberOfPropertiesSet > 1) throw new System.ArgumentException("Multiple union values set");
+
+    }
+  }
+}
