DynamoDbEncryption/runtimes/net/Generated/JsonEncryptor/DecryptAs.cs
@@ -1,0 +1,35 @@
+// Copyright Amazon.com Inc. or its affiliates. All Rights Reserved.
+// SPDX-License-Identifier: Apache-2.0
+// Do not modify this file. This file is machine generated, and any changes to it will be overwritten.
+using System;
+using AWS.Cryptography.DbEncryptionSDK.DynamoDb.Json;
+namespace AWS.Cryptography.DbEncryptionSDK.DynamoDb.Json
+{
+  public class DecryptAs
+  {
+    private string _encrypt;
+    private string _decrypt;
+    public string Encrypt
+    {
+      get { return this._encrypt; }
+      set { this._encrypt = value; }
+    }
+    public bool IsSetEncrypt()
+    {
+      return this._encrypt != null;
+    }
+    public string Decrypt
+    {
+      get { return this._decrypt; }
+      set { this._decrypt = value; }
+    }
+    public bool IsSetDecrypt()
+    {
+      return this._decrypt != null;
+    }
+    public void Validate()
+    {
+
+    }
+  }
+}
