DynamoDbEncryption/runtimes/net/Generated/JsonEncryptor/JsonEncryptorConfig.cs
@@ -8,8 +8,11 @@ namespace AWS.Cryptography.DbEncryptionSDK.DynamoDb.Json
   public class JsonEncryptorConfig
   {
     private string _logicalTableName;
-    private AWS.Cryptography.DbEncryptionSDK.DynamoDb.Json.Actions _actions;
+    private System.Collections.Generic.Dictionary<string, AWS.Cryptography.DbEncryptionSDK.DynamoDb.Json.Action> _attributeActionsOnEncrypt;
+    private System.Collections.Generic.List<string> _allowedUnsignedAttributes;
+    private string _allowedUnsignedAttributePrefix;
     private AWS.Cryptography.DbEncryptionSDK.DynamoDb.Json.DbesdkEncrypt _encrypt;
+    private System.Collections.Generic.List<string> _decryptAs;
     public string LogicalTableName
     {
       get { return this._logicalTableName; }
@@ -19,14 +22,32 @@ namespace AWS.Cryptography.DbEncryptionSDK.DynamoDb.Json
     {
       return this._logicalTableName != null;
     }
-    public AWS.Cryptography.DbEncryptionSDK.DynamoDb.Json.Actions Actions
+    public System.Collections.Generic.Dictionary<string, AWS.Cryptography.DbEncryptionSDK.DynamoDb.Json.Action> AttributeActionsOnEncrypt
     {
-      get { return this._actions; }
-      set { this._actions = value; }
+      get { return this._attributeActionsOnEncrypt; }
+      set { this._attributeActionsOnEncrypt = value; }
     }
-    public bool IsSetActions()
+    public bool IsSetAttributeActionsOnEncrypt()
     {
-      return this._actions != null;
+      return this._attributeActionsOnEncrypt != null;
+    }
+    public System.Collections.Generic.List<string> AllowedUnsignedAttributes
+    {
+      get { return this._allowedUnsignedAttributes; }
+      set { this._allowedUnsignedAttributes = value; }
+    }
+    public bool IsSetAllowedUnsignedAttributes()
+    {
+      return this._allowedUnsignedAttributes != null;
+    }
+    public string AllowedUnsignedAttributePrefix
+    {
+      get { return this._allowedUnsignedAttributePrefix; }
+      set { this._allowedUnsignedAttributePrefix = value; }
+    }
+    public bool IsSetAllowedUnsignedAttributePrefix()
+    {
+      return this._allowedUnsignedAttributePrefix != null;
     }
     public AWS.Cryptography.DbEncryptionSDK.DynamoDb.Json.DbesdkEncrypt Encrypt
     {
@@ -37,10 +58,20 @@ namespace AWS.Cryptography.DbEncryptionSDK.DynamoDb.Json
     {
       return this._encrypt != null;
     }
+    public System.Collections.Generic.List<string> DecryptAs
+    {
+      get { return this._decryptAs; }
+      set { this._decryptAs = value; }
+    }
+    public bool IsSetDecryptAs()
+    {
+      return this._decryptAs != null;
+    }
     public void Validate()
     {
       if (!IsSetLogicalTableName()) throw new System.ArgumentException("Missing value for required property 'LogicalTableName'");
-      if (!IsSetActions()) throw new System.ArgumentException("Missing value for required property 'Actions'");
+      if (!IsSetAttributeActionsOnEncrypt()) throw new System.ArgumentException("Missing value for required property 'AttributeActionsOnEncrypt'");
+      if (!IsSetEncrypt()) throw new System.ArgumentException("Missing value for required property 'Encrypt'");
 
     }
   }
