DynamoDbEncryption/dafny/JsonEncryptor/src/foo.dfy
@@ -1,7 +1,7 @@
 include "Util.dfy"
 include "JsonToStruct.dfy"
 
-module Foo {
+module {:options "-functionSyntax:4"} Foo {
 
   import opened StandardLibrary
   import opened JsonEncryptorUtil
@@ -10,6 +10,7 @@ module Foo {
   import CSE = AwsCryptographyDbEncryptionSdkStructuredEncryptionTypes
   import opened Wrappers
   import JsonToStruct
+  import opened JSON.Values
 
   datatype Config = Config(
     nameonly logicalTableName : string,
@@ -24,11 +25,42 @@ module Foo {
 
   type InternalConfig = Config
 
+  opaque function {:opaque} {:fuel 0,0} SmithyJsonToObject2(item : Json) : (res :Result<JSON, string>)
+    ensures res.Success? ==> res.value.Object?
+  {
+    var json :- if item.text? then
+      JsonToStruct.StringToJson(item.text)
+    else
+      JsonToStruct.Utf8ToJson(item.utf8);
+
+    // :- Need(json.Object?, "JSON to encrypt/decrypt must be an Object : " + JsonToStruct.SmithyJsonToString(item));
+    :- Need(json.Object?, "bad");
+    Success(json)
+  }
+
+  opaque function SmithyJsonToObject4(item : Json) : (res :Result<JSON, string>)
+    // ensures res.Success? ==> res.value.Object?
+  {
+    Failure("foo")
+  }
+
+  method SmithyJsonToObject3(item : Json) returns (res :Result<JSON, string>)
+    ensures res.Success? ==> res.value.Object?
+  {
+    var json :- if item.text? then
+      JsonToStruct.StringToJson(item.text)
+    else
+      JsonToStruct.Utf8ToJson(item.utf8);
+
+    :- Need(json.Object?, "JSON to encrypt/decrypt must be an Object : " + JsonToStruct.SmithyJsonToString(item));
+    return Success(json);
+  }
+
   // method {:vcs_split_on_every_assert} EncryptObject2(config: InternalConfig, input: EncryptObjectInput)
   method EncryptObject2(input: EncryptObjectInput)
   {
-    //var origJson := JsonToStruct.SmithyJsonToObject(input.plaintextObject).MapFailure(e => E(e));
-    var origJson := JsonToStruct.SmithyJsonToObject(input.plaintextObject);
+    //var origJson := JsonToStruct.SmithyJsonToObject2(input.plaintextObject).MapFailure(e => E(e));
+    var origJson := SmithyJsonToObject2(input.plaintextObject);
     assert 3 == 3;
   }
 
